Added some basic instantiations for list_scene_space

Alphabet_Scene_Spaces.thy
@@ -38,6 +38,37 @@ qed
 
 end
 
+instantiation unit :: list_scene_space
+begin
+
+definition VarList_unit :: "unit scene list" where [simp]: "VarList_unit = []"
+
+instance
+  by (intro_classes, simp_all add: scene_indeps_def scene_span_def unit_scene_top_eq_bot)
+
+end
+
+instantiation prod :: (list_scene_space, list_scene_space) list_scene_space
+begin
+
+definition VarList_prod :: "('a \<times> 'b) scene list" where "VarList_prod = map (\<lambda> x. x ;\<^sub>S fst\<^sub>L) VarList @ map (\<lambda> x. x ;\<^sub>S snd\<^sub>L) VarList"
+
+instance proof
+  have pw: "pairwise (\<bowtie>\<^sub>S) (set (map (\<lambda> x. x ;\<^sub>S fst\<^sub>L) VarList @ map (\<lambda> x. x ;\<^sub>S snd\<^sub>L) VarList))"
+    by (auto simp add: pairwise_def Vars_ext_lens_indep scene_comp_pres_indep scene_indep_sym Vars_VarList)
+  show "\<And>x:: ('a \<times> 'b) scene. x \<in> set VarList \<Longrightarrow> idem_scene x"
+    by (auto simp add: VarList_prod_def Vars_VarList)
+  from pw show "scene_indeps (set (VarList :: ('a \<times> 'b) scene list))"
+    by (simp add: VarList_prod_def scene_indeps_def Vars_VarList)
+  show "scene_span (set (VarList :: ('a \<times> 'b) scene list))"
+    by (simp only: scene_span_def VarList_prod_def pw map_lcomp_Vars_is_lens fst_vwb_lens snd_vwb_lens Vars_VarList)
+       (simp add: VarList_prod_def Vars_VarList Vars_prod_def map_lcomp_def top_scene_eq)
+  show "Vars = (set (VarList :: ('a \<times> 'b) scene list))"
+    by (simp add: VarList_prod_def Vars_prod_def map_lcomp_def Vars_VarList)
+qed  
+
+end
+
 abbreviation foldr_scene :: "'a scene list \<Rightarrow> 'a scene" ("foldr\<^sub>S") where
 "foldr_scene as \<equiv> foldr (\<squnion>\<^sub>S) as \<bottom>\<^sub>S"
 
